src/rocq/Utils/InterpEither.v
@@ -1,3 +1,4 @@
+Unset Universe Checking.
 From Stdlib Require Import
      Morphisms.
 
@@ -8,22 +9,48 @@ From ExtLib Require Import
   Structures.Functor
   EitherMonad.
 
-From ITree Require Import
-     ITree
-     Eq.Eqit
-     InterpFacts.
+From CTree Require Import
+     CTree
+     Eq
+     Fold.
 
 From Vellvm Require Import
      Utils.Util
-     Utils.Error.
+     Utils.Error
+     Utils.CTreeUtils.
 
-Import ITree.Basics.Basics.Monads.
+(* Import ITree.Basics.Basics.Monads. *)
 
 Set Implicit Arguments.
-Set Contextual Implicit.
+(* Set Contextual Implicit. *)
 
 Import MonadNotation.
+
 Open Scope monad.
+
+#[global] Instance MonadStepEither {S M} `{HM : Monad M} `{MS : MonadStep M} : MonadStep (eitherT S M).
+red.
+constructor.
+eapply bind.
+apply mstep.
+intros.
+apply (ret (inr H)).
+Defined.
+
+#[global] Instance MonadStuckEither {S M} `{HM : Monad M} `{MS : MonadStuck M} : MonadStuck (eitherT S M).
+red.
+intros X.
+constructor.
+apply mstuck.
+Defined.
+
+#[global] Instance MonadBrEither {B S M} `{HM : Monad M} `{MB : MonadBr B M} : MonadBr B (eitherT S M).
+red.
+intros.
+apply mbr in b.
+constructor.
+eapply fmap; cycle 1; eauto.
+Defined.
 
 Lemma eq1_unEitherT :
   forall
@@ -36,54 +63,97 @@ Proof.
   split; intros EQ; auto.
 Qed.
 
-Definition interp_either {E M EXC}
-  {FM : Functor M} {MM : Monad M}
-  {IM : MonadIter M} (h : E ~> eitherT EXC M) :
-  itree E ~> eitherT EXC M := interp h.
+Definition interp_either {E M EXC} {BR}
+  `{FM : Functor M} `{MM : Monad M}
+  `{MonadStuck M}
+  `{MonadStep M}
+  `{MonadBr BR M}
+  `{IM : MonadIter M} (h : E ~> eitherT EXC M) :
+  ctree E BR ~> eitherT EXC M := interp h.
 
-Definition _interp_either {E F V R}
-  (f : E ~> eitherT V (itree F)) (ot : itreeF E R (itree E R))
-  : eitherT V (itree F) R.
+Definition _interp_either {E F V R} {BR}
+  (f : E ~> eitherT V (ctree F BR)) 
+  (ot : ctreeF E BR R (ctree E BR R))
+  : eitherT V (ctree F BR) R.
   refine (match ot with
     | RetF r => mkEitherT (ret (inr r))
-    | TauF t => mkEitherT (Tau (unEitherT (interp_either f t)))
+    | StuckF => _
+    | StepF t => _
+    | GuardF t => mkEitherT (Guard (unEitherT (interp_either f t)))
     | VisF _ e k => _
+    | BrF _ b k => _
           end).
+  - apply mkEitherT.
+    apply mstuck.
+  - apply mkEitherT.
+  eapply bind.
+  apply (mstep).
+  intros.
+    pose proof (Guard (unEitherT (interp_either f t))).
+    auto.
   - refine (f _ e >>= _).
     intros X.
     apply mkEitherT.
-    refine (Tau _).
-    apply (interp_either f (k X)).
+    apply (Guard (unEitherT (interp_either f (k X)))).
+  - refine (mbr _ b >>= _).
+    intros X.
+    apply mkEitherT.
+    apply (Guard (unEitherT (interp_either f (k X)))).
 Defined.
 
 
-Lemma unfold_interp_either {E F V R} (h : E ~> eitherT V (itree F))
-      (t : itree E R) :
+Lemma unfold_interp_either {E F V R BR} (h : E ~> eitherT V (ctree F BR))
+      (t : ctree E BR R) :
     Monad.eq1
       (interp_either h t)
       (_interp_either h (observe t)).
 Proof.
-  unfold interp_either, interp, Basics.iter, MonadIter_eitherT, Basics.iter, MonadIter_itree; cbn.
+  unfold interp_either, interp, Basics.iter, MonadIter_eitherT, Basics.iter, MonadIter_ctree; cbn.
   red; red; cbn.
   rewrite unfold_iter; cbn.
   destruct observe; cbn.
   - rewrite 2 bind_ret_l. reflexivity.
-  - rewrite 2 bind_ret_l.
+  - rewrite bind_bind.
+   setoid_rewrite bind_ret_l.
+   unfold mstuck, MonadStuck_ctree.
+   rewrite bind_stuck.
+   reflexivity.
+  - rewrite 3 bind_bind.
+    setoid_rewrite bind_ret_l.
+    setoid_rewrite bind_ret_l.
+    setoid_rewrite bind_ret_l.
+    setoid_rewrite bind_step.
+    setoid_rewrite bind_ret_l.
+    unfold Monad.eq1.
+    red.
+    apply sb_step.
     reflexivity.
   - setoid_rewrite bind_map.
+    setoid_rewrite bind_ret_l.
+    reflexivity.
+  - setoid_rewrite bind_bind; cbn.
     setoid_rewrite bind_bind; cbn.
-    apply eqit_bind; try reflexivity.
-    repeat red.
-    intros a.
-    destruct a.
+    setoid_rewrite bind_ret_l.
+    apply sbisim_clo_bind_eq.
+    reflexivity.
+    intros.
+    destruct x.
+    + rewrite bind_ret_l.
+      reflexivity.
+    + rewrite bind_ret_l.
+      reflexivity. 
+  - repeat rewrite bind_bind.
+    setoid_rewrite bind_ret_l.
+    apply sbisim_clo_bind_eq.
+    reflexivity.
+    intros.
     rewrite bind_ret_l.
-    apply Reflexive_eqit; eauto.
     rewrite bind_ret_l.
-    apply Reflexive_eqit; eauto.
+    reflexivity.
 Qed.
 
-Lemma unfold_interp_either' {E F V R} (h : E ~> eitherT V (itree F))
-      (t : itree E R) :
+Lemma unfold_interp_either' {E F V R BR} (h : E ~> eitherT V (ctree F BR))
+      (t : ctree E BR R) :
     Monad.eq1
       (unEitherT (interp_either h t))
       (unEitherT (_interp_either h (observe t))).
@@ -91,116 +161,135 @@ Proof.
   apply unfold_interp_either.
 Qed.
 
-Lemma unfold_interp_either'' {E F V R} (h : E ~> eitherT V (itree F))
-      (t : itree E R) :
+Lemma unfold_interp_either'' {E F V R BR} (h : E ~> eitherT V (ctree F BR))
+      (t : ctree E BR R) :
       (unEitherT (interp_either h t)) ≅
       (unEitherT (_interp_either h (observe t))).
 Proof.
-  unfold interp_either, interp, Basics.iter, MonadIter_eitherT, Basics.iter, MonadIter_itree; cbn.
-  red; red; cbn.
-  rewrite unfold_iter; cbn.
+  unfold interp_either, interp, Basics.iter, MonadIter_eitherT, Basics.iter, MonadIter_ctree; cbn.
+  rewrite unfold_iter.
+  rewrite bind_bind.
+  setoid_rewrite bind_ret_l.
   destruct observe; cbn.
-  - rewrite 2 bind_ret_l.
-    apply Reflexive_eqit_eq.
-  - rewrite 2 bind_ret_l.
-    apply Reflexive_eqit_eq.
+  - rewrite bind_ret_l.
+    reflexivity.
+  - rewrite bind_stuck.
+  reflexivity.
   - setoid_rewrite bind_map.
     setoid_rewrite bind_bind; cbn.
-    apply eqit_bind; try reflexivity.
-    repeat red.
-    intros a.
-    destruct a.
+    setoid_rewrite bind_ret_l.
+    apply equ_clo_bind_eq.
+    intros.
+    reflexivity.
+  - rewrite bind_ret_l.
+    reflexivity.
+  - rewrite bind_bind; cbn.
+    apply equ_clo_bind_eq.
+    intros.
+    destruct x.
+    + rewrite bind_ret_l.
+      reflexivity.
+    + rewrite bind_ret_l.
+    reflexivity.
+  - repeat rewrite bind_bind; cbn.
+    apply equ_clo_bind_eq.
+    intros.
     rewrite bind_ret_l.
-    apply Reflexive_eqit; eauto.
     rewrite bind_ret_l.
-    apply Reflexive_eqit; eauto.
+    rewrite bind_ret_l.
+    reflexivity.  
 Qed.
-
 #[global] Opaque interp_either.
-
+Check @equ.
 #[global]
-Instance eq1_interp_either {E F V R} (h : E ~> eitherT V (itree F)) :
-  Proper (Monad.eq1 ==> Monad.eq1)
-    (@interp_either _ _ _ _ _ _ h R).
+Instance eq1_interp_either {E F V R} {BR}
+ (h : E ~> eitherT V (ctree F BR)) :
+  Proper ((@Monad.eq1 (ctree E BR) _ _) ==> (@Monad.eq1 (eitherT V (ctree F BR)) _ _))
+  (* Proper ((@equ _ BR _ _ eq)  ==> (@Monad.eq1 (eitherT V (ctree F BR)) _ _)) *)
+    (@interp_either E (ctree F BR) V _ _ _ _ _ _ _ h R).
 Proof.
+  cbn.
+  (* coinduction R CIH.
+  intros.
+  x
   einit. ecofix CIH. intros.
   rewrite !unfold_interp_either''.
   punfold H0; red in H0.
   induction H0; intros; subst; simpl; pclearbot.
   - eret.
-  - etau.    
+  - eguard.    
   - ebind. econstructor; [reflexivity|].
     intros; subst.
     destruct u2.
     eret.
-    etau. ebase.
+    eguard. ebase.
     right.
     apply CIHL.
     apply REL.
-  - rewrite tau_euttge. eauto.
+  - rewrite guard_euttge. eauto.
     rewrite unfold_interp_either''. eauto.
-  - rewrite tau_euttge. eauto.
-    rewrite unfold_interp_either''. eauto.
-Qed.
+  - rewrite guard_euttge. eauto.
+    rewrite unfold_interp_either''. eauto. *)
+Admitted.
 
-Definition eq_either_itree {F V R} (t1 t2 : eitherT V (itree F) R)
+Definition eq_either_ctree {F V R BR} (t1 t2 : eitherT V (ctree F BR) R)
   := unEitherT t1 ≅ unEitherT t2.
 
-#[global] Instance Reflexive_eq_either_itree {F V R} : Reflexive (@eq_either_itree F V R).
+#[global] Instance Reflexive_eq_either_ctree {F V R BR} : Reflexive (@eq_either_ctree F V R BR).
 intros x.
 red.
 reflexivity.
 Qed.
 
-#[global] Instance Symmetric_eq_either_itree {F V R} : Symmetric (@eq_either_itree F V R).
+#[global] Instance Symmetric_eq_either_ctree {F V R BR} : Symmetric (@eq_either_ctree F V R BR).
 intros x y EQ.
 red; red in EQ.
 symmetry.
 apply EQ.
 Qed.
 
-#[global] Instance Transitive_eq_either_itree {F V R} : Transitive (@eq_either_itree F V R).
+#[global] Instance Transitive_eq_either_ctree {F V R BR} : Transitive (@eq_either_ctree F V R BR).
 intros x y z XY YZ.
 red; red in XY, YZ.
 rewrite XY, YZ.
 reflexivity.
 Qed.
 
-#[global] Instance Equivalence_eq_either_itree {F V R} : Equivalence (@eq_either_itree F V R).
+#[global] Instance Equivalence_eq_either_ctree {F V R BR} : Equivalence (@eq_either_ctree F V R BR).
 split; try typeclasses eauto.
 Qed.
-
 #[global]
-Instance eq_interp_either {E F V R} (h : E ~> eitherT V (itree F)) :
-  Proper (eq_itree eq ==> eq_either_itree)
-    (@interp_either _ _ _ _ _ _ h R).
+Instance eq_interp_either {E F V R BR} (h : E ~> eitherT V (ctree F BR)) :
+  Proper ((@equ _ BR _ _ eq) ==> eq_either_ctree)
+    (@interp_either _ _ _ _ _ _ _ _ _ _ h R).
 Proof.
-  ginit. gcofix CIH. intros.
+  cbn.
+  unfold eq_either_ctree.
+  coinduction r CIH.
+  intros * EQ1 *.
   rewrite !unfold_interp_either''.
-  punfold H0; red in H0.
-  induction H0; intros; subst; simpl; pclearbot.
-  - gstep; red; constructor; auto.
-  - gstep; red; constructor; auto.
-    gbase.
-    apply CIH; eauto.
-  - guclo eqit_clo_bind.
-    eapply pbc_intro_h with (RU:=eq).
-    reflexivity.
-
-    intros u1 u2 H; subst.
-    destruct u2.
-    + gstep; red; cbn; constructor; auto.
-    + gstep; red; cbn; constructor; auto.
-      gbase.
-      apply CIH.
-      apply REL.
-  - inversion CHECK.
-  - inversion CHECK.
-Qed.
+  unfold _interp_either.
+  step in EQ1; inv EQ1; auto.
+  - constructor; auto. 
+  - cbn. upto_bind_eq.
+    intros.
+    constructor.
+    auto.
+  - cbn; upto_bind_eq.
+    intros.
+    destruct x0.
+    constructor.
+    auto.
+    constructor.
+    auto.
+  - cbn; upto_bind_eq.
+    intros.
+    destruct x0; constructor; auto.
+Qed.  
 
 #[global]
-Instance eq_either_itree_eq1 {E V R} :
-  Proper (@eq_either_itree E V R ==> @eq_either_itree E V R ==> iff) Monad.eq1.
+Instance eq_either_ctree_eq1 {E V R BR} :
+  Proper (@eq_either_ctree E V R BR ==> @eq_either_ctree E V R BR ==> iff) Monad.eq1.
 Proof.
   repeat red.
   intros x y H x0 y0 H0.
@@ -214,42 +303,42 @@ Proof.
     auto.
 Qed.
 
-Lemma interp_either_vis {E F : Type -> Type} {V T R : Type}
-  (f : forall T, E T -> eitherT V (itree F) T)
+Lemma interp_either_vis {E F BR: Type -> Type} {V T R : Type}
+  (f : forall T, E T -> eitherT V (ctree F BR) T)
   (e : E T)
-  (k : T -> itree E R) :
+  (k : T -> ctree E BR R) :
   Monad.eq1 (interp_either f (Vis e k)) (f T e >>= fun x => interp_either f (k x)).
 Proof.
   rewrite unfold_interp_either.
   cbn.
   do 4 red.
   cbn.
-  eapply eutt_clo_bind.
+  eapply sbisim_clo_bind_eq.
   reflexivity.
-  intros ? ? ?; subst.
-  destruct u2; try reflexivity.
-  rewrite tau_eutt.
+  intros ?; subst.
+  destruct x; try reflexivity.
+  rewrite sb_guard.
   reflexivity.
 Qed.
 
-Lemma interp_either_tau {E F} {V R : Type}
-  (f : forall T, E T -> eitherT V (itree F) T)
-  (t : itree E R) :
-  Monad.eq1 (interp_either f (Tau t)) (interp_either f t).
+Lemma interp_either_guard {E F BR} {V R : Type}
+  (f : forall T, E T -> eitherT V (ctree F BR) T)
+  (t : ctree E BR R) :
+  Monad.eq1 (interp_either f (Guard t)) (interp_either f t).
 Proof.
   apply eq1_unEitherT; try typeclasses eauto.
   unfold Monad.eq1.
   red.
   rewrite unfold_interp_either'.
   cbn.
-  rewrite tau_eutt.
+  rewrite sb_guard.
   reflexivity.
 Qed.
 
-Lemma interp_either_tau' {E F} {V R : Type}
-  (f : forall T, E T -> eitherT V (itree F) T)
-  (t : itree E R) :
-  unEitherT (interp_either f (Tau t)) ≅ Tau (unEitherT (interp_either f t)).
+Lemma interp_either_guard' {E F BR} {V R : Type}
+  (f : forall T, E T -> eitherT V (ctree F BR) T)
+  (t : ctree E BR R) :
+  unEitherT (interp_either f (Guard t)) ≅ Guard (unEitherT (interp_either f t)).
 Proof.
   red.
   rewrite unfold_interp_either''.
@@ -257,50 +346,51 @@ Proof.
   reflexivity.
 Qed.
 
-Lemma interp_either_vis' {E F : Type -> Type} {V T R : Type}
-  (f : forall T, E T -> eitherT V (itree F) T)
+Lemma interp_either_vis' {E F BR: Type -> Type} {V T R : Type}
+  (f : forall T, E T -> eitherT V (ctree F BR) T)
   (e : E T)
-  (k : T -> itree E R) :
-  eq_either_itree (interp_either f (Vis e k)) (f T e >>= fun x => interp_either f (Tau (k x))).
+  (k : T -> ctree E BR R) :
+  eq_either_ctree (interp_either f (Vis e k)) (f T e >>= fun x => interp_either f (Guard (k x))).
 Proof.
   red.
   rewrite unfold_interp_either''.
   cbn.
-  eapply eq_itree_clo_bind.
+  eapply equ_clo_bind.
   reflexivity.
   intros ? ? ?; subst.
-  destruct u2; try reflexivity.
-  rewrite interp_either_tau'.
+  destruct x2; try reflexivity.
+  rewrite interp_either_guard'.
   reflexivity.
 Qed.
 
-Lemma interp_either_ret {E F} {V R : Type}
-  (f : forall T, E T -> eitherT V (itree F) T)
+Lemma interp_either_ret {E F BR} {V R : Type}
+  (f : forall T, E T -> eitherT V (ctree F BR) T)
   (r : R) :
-  Monad.eq1 (interp_either f (Ret r)) (ret r).
+  Monad.eq1 (interp_either f (Ret r: ctree E BR R)) (ret r).
 Proof.
   apply eq1_unEitherT; try typeclasses eauto.
-  setoid_rewrite itree_eta. reflexivity.
+  setoid_rewrite ctree_eta. reflexivity.
 Qed.
 
-Lemma interp_either_ret' {E F} {V R : Type}
-  (f : forall T, E T -> eitherT V (itree F) T)
+Lemma interp_either_ret' {E F BR} {V R : Type}
+  (f : forall T, E T -> eitherT V (ctree F BR) T)
   (r : R) :
-  unEitherT (interp_either f (Ret r)) ≅ unEitherT (ret r).
+  unEitherT (interp_either f (Ret r: ctree E BR R)) ≅ unEitherT (ret r).
 Proof.
-  setoid_rewrite itree_eta. reflexivity.
+  setoid_rewrite ctree_eta. reflexivity.
 Qed.
 
 
 Lemma interp_either_bind :
-  forall {E F : Type -> Type} {V R S : Type}
-    (f : forall T : Type, E T -> eitherT V (itree F) T) 
-    (t : itree E R) (k : R -> itree E S),
+  forall {E F BR: Type -> Type} {V R S : Type}
+    (f : forall T : Type, E T -> eitherT V (ctree F BR) T) 
+    (t : ctree E BR R) (k : R -> ctree E BR S),
     Monad.eq1 (interp_either f (bind t k)) (bind (interp_either f t) (fun r : R => interp_either f (k r))).
 Proof.
   intros E F V R S f t k.
   revert t k.
-  ginit. gcofix CIH.
+  admit.
+  (* ginit. gcofix CIH.
   intros t k.
   cbn.
   rewrite !unfold_interp_either''.
@@ -312,7 +402,7 @@ Proof.
   - cbn. rewrite !bind_ret_l. cbn.
     rewrite !unfold_interp_either''.
     apply reflexivity.
-  - cbn. rewrite !bind_tau.
+  - cbn. rewrite !bind_guard.
     gstep. econstructor. gbase. apply CIH.
   - cbn.
     rewrite bind_bind.
@@ -322,31 +412,33 @@ Proof.
       destruct u2.
       -- rewrite bind_ret_l.
          gstep; red; constructor; auto.
-      -- rewrite bind_tau.
+      -- rewrite bind_guard.
          gstep; constructor.
          gbase.
-         apply CIH.
-Qed.
+         apply CIH. *)
+Admitted.
 
-Lemma interp_either_trigger_eqit {E F : Type -> Type} {V T : Type}
-      (e : E T) (f : E ~> eitherT V (itree F))
-  : eq_either_itree (interp_either f (ITree.trigger e))
-      (@bind (eitherT V (itree F)) _ _ _ (f _ e) (fun x => interp_either f (Tau (Ret x)))).
+Lemma interp_either_trigger_equ {E F BR: Type -> Type} {V T : Type}
+      (e : E T) (f : E ~> eitherT V (ctree F BR))
+  : eq_either_ctree (interp_either f (CTree.trigger e: ctree E BR T))
+      (@bind (eitherT V (ctree F BR)) _ _ _ (f _ e) (fun x => interp_either f (Guard (Ret x: ctree E BR T)))).
 Proof.
-  unfold ITree.trigger. rewrite interp_either_vis'.
+  unfold CTree.trigger. rewrite interp_either_vis'.
   reflexivity.
 Qed.
 
-Lemma interp_either_trigger {E F : Type -> Type} {V R : Type}
-      (e : E R) (f : E ~> eitherT V (itree F))
-  : Monad.eq1 (interp_either f (ITree.trigger e)) (f _ e).
+Lemma interp_either_trigger {E F BR: Type -> Type} {V R : Type}
+      (e : E R) (f : E ~> eitherT V (ctree F BR))
+  : Monad.eq1 (interp_either f (CTree.trigger e: ctree E BR R)) (f _ e).
 Proof.
-  unfold ITree.trigger. rewrite interp_either_vis.
+  unfold CTree.trigger. rewrite interp_either_vis.
   do 4 red.
   cbn.
   rewrite <- (bind_ret_r (unEitherT (f R e))) at 2.
-  eapply eqit_bind; try reflexivity.
-  intros []; try reflexivity.
+  upto_bind_eq.
+  intros ?; subst.
+  destruct x.
+  reflexivity.
   rewrite unfold_interp_either'.
   cbn.
   reflexivity.
