src/rocq/Handlers/CTreeHandler.v
@@ -1,0 +1,126 @@
+(** * Event handlers *)
+
+(** Events types [E, F : Type -> Type] and itree [E ~> itree F]
+    form a category. *)
+
+(* begin hide *)
+From Coq Require Import
+     Morphisms.
+
+From CTree Require Import
+    CTree
+    Fold
+    Eq
+    WBisim.
+
+Import Relation.
+Import CategoryOps.
+(* end hide *)
+
+(** ** Handler combinators *)
+
+Module Handler.
+(** These are defined primarily for documentation. Except for [htrigger],
+    it is recommended to use the [CategoryOps] classes instead
+    (with the same function names). *)
+
+(** Lift an _event morphism_ into an _event handler_. *)
+Definition htrigger {A B} {BR} (m : A ~> B) : A ~> ctree B BR :=
+  fun _ e => CTree.trigger (m _ e).
+
+(** Trivial handler, triggering any event it's given, so
+    the resulting interpretation is the identity function:
+    [interp (id_ E) _ t ≈ t]. *)
+Definition id_ (E : Type -> Type) {BR} : E ~> ctree E BR := CTree.trigger.
+
+(** Chain handlers: [g] handles the events produced by [f]. *)
+Definition cat {E F G : Type -> Type} {BR}
+           (f : E ~> ctree F BR) (g : F ~> ctree G BR)
+  : E ~> ctree G BR
+  := fun R e => interp g (f R e).
+
+(** Wrap events to the left of a sum. *)
+Definition inl_ {E F : Type -> Type} {BR} : E ~> ctree (E +' F) BR
+  := htrigger inl1.
+
+(** Wrap events to the right of a sum. *)
+Definition inr_ {E F : Type -> Type} {BR}: F ~> ctree (E +' F) BR
+  := htrigger inr1.
+
+(** Case analysis on sums of events. *)
+Definition case_ {E F G : Type -> Type} {BR}
+           (f : E ~> ctree G BR) (g : F ~> ctree G BR)
+  : E +' F ~> ctree G BR
+  := fun _ ab => match ab with
+                 | inl1 a => f _ a
+                 | inr1 b => g _ b
+                 end.
+
+(* Definition case_' {E F G : Type -> Type}
+           (f : E ~> ctree G) (g : F ~> ctree G)
+  : E +' F ~> ctree G
+  := @case_sum1 E F (ctree G) f g.
+(* TODO: why is there a universe inconsistency if this is before [inl_] and [inr_]? *)
+ *)
+
+(** Handle events independently, with disjoint sets of output events. *)
+Definition bimap {E F G H : Type -> Type} {BR}
+           (f : E ~> ctree G BR) (g : F ~> ctree H BR)
+  : E +' F ~> ctree (G +' H) BR
+  := case_ (Handler.cat f inl_) (Handler.cat g inr_).
+
+(** Handle [void1] events (of which there are none). *)
+Definition empty {E : Type -> Type} {BR}
+  : void1 ~> ctree E BR
+  := fun _ e => match e : void1 _ with end.
+
+End Handler.
+
+(** ** Category instances *)
+Definition Handler (E F : Type -> Type) BR := E ~> ctree F BR.
+
+(** Conversion functions between [Handler] and [_ ~> ctree _].
+    Although they are the identity function, they guide type inference
+    and type class search. *)
+Definition handle {E F} {BR} (f : Handler E F BR) : E ~> ctree F BR := f.
+Definition handling {E F} {BR} (f : E ~> ctree F BR) : Handler E F BR := f.
+
+Definition eq_Handler {E F : Type -> Type} {BR}
+  : Handler E F BR -> Handler E F BR -> Prop
+  := i_pointwise (fun R => sbisim eq).
+
+Definition eutt_Handler {E F : Type -> Type} {BR}
+  : Handler E F BR -> Handler E F BR -> Prop
+  := i_pointwise (fun R => wbisim ).
+(** The default handler equivalence is [eutt]. *)
+#[global]
+Instance Eq2_Handler BR: Eq2 (fun a b => (Handler a b BR))
+  := (fun e f => (@eutt_Handler e f BR)).
+
+#[global]
+Instance Id_Handler BR: Id_ (fun a b => (Handler a b BR))
+  := (fun e => (@Handler.id_ e BR)).
+
+#[global]
+Instance Cat_Handler BR: Cat (fun a b => (Handler a b BR))
+  := (fun e f g => (@Handler.cat e f g BR)).
+
+#[global]
+Instance Case_sum1_Handler BR: Case (fun a b => (Handler a b BR)) sum1
+  := (fun e f g => (@Handler.case_ e f g BR)).
+
+#[global]
+Instance Inl_sum1_Handler BR: Inl (fun a b => (Handler a b BR)) sum1
+  := (fun e f => @Handler.inl_ e f BR).
+
+#[global]
+Instance Inr_sum1_Handler BR: Inr (fun a b => (Handler a b BR)) sum1
+  := (fun e f => @Handler.inr_ e f BR).
+
+#[global]
+Instance Initial_void1_Handler BR: Initial (fun a b => (Handler a b BR)) void1
+  := (fun e => @Handler.empty e BR).
+
+(* #[global]
+Instance Iter_Handler BR: Iter (fun a b => (Handler a b BR)) sum1
+  := @mrec. *)
