src/rocq/Semantics/Memory/ErrSID.v
@@ -1,3 +1,4 @@
+Unset Universe Checking.
 From Stdlib Require Import ZArith String.
 
 From ExtLib Require Import
