src/rocq/Theory/DenotationTheory.v
@@ -15,7 +15,7 @@ From Vellvm Require Import
      Semantics
      Syntax.ScopeTheory
      Utils.PostConditions
-     Utils.ITreeRaise.
+     .
 
 #[export] Remove Hints Eqv.EqvWF_Build : typeclass_instances.
 
